Started using the modular types.

Java/src/Java/Func/JavaType.v
@@ -1,555 +1,112 @@
 Require Import ExtLib.Core.RelDec.
 Require Import ExtLib.Data.Fun.
+Require Import ExtLib.Data.POption.
 Require Import ExtLib.Tactics.
 
 Require Import MirrorCore.TypesI.
+Require Import MirrorCore.MTypes.ModularTypes.
+Require Import MirrorCore.Views.FuncView.
 
-Require Import Charge.Views.ILogicView.
-Require Import Charge.Views.BILogicView.
-Require Import Charge.Views.EmbedView.
 Require Import ChargeCore.Open.Subst.
-Require Import ChargeCore.Logics.ILInsts.
-Require Import ChargeCore.Logics.BILInsts.
-Require Import ChargeCore.Logics.ILogic.
-Require Import ChargeCore.Logics.Later.
 
 Require Import Java.Logic.AssertionLogic.
 Require Import Java.Logic.SpecLogic.
 Require Import Java.Language.Lang.
 Require Import Java.Language.Program.
 
-Require Import Coq.Strings.String.
-Require Import Coq.Bool.Bool.
-
 Set Implicit Arguments.
 Set Strict Implicit.
 
-Inductive typ : Type :=
-| tyArr : typ -> typ -> typ
-| tyList : typ -> typ
-| tyProd : typ -> typ -> typ
-| tyBool : typ
-| tyVal : typ
-| tyString : typ
-| tyNat : typ
-| tyProp : typ
-| tySpec : typ
-| tyAsn : typ
-| tyProg : typ
-| tyMethod : typ
-| tyCmd : typ
-| tyDExpr : typ
-| tySubst : typ.
+Universe U.
 
-Notation "'tyStack'" := (tyArr tyString tyVal).
+Inductive java_typ : nat -> Type@{U} :=
+| tVal : java_typ 0
+| tSpec : java_typ 0
+| tAsn : java_typ 0
+| tProg : java_typ 0
+| tMethod : java_typ 0
+| tCmd : java_typ 0
+| tExpr : java_typ 0
+| tSubst : java_typ 0.
 
-Notation "'tyPure'" := (tyArr tyStack tyProp).
-Notation "'tySasn'" := (tyArr tyStack tyAsn).
-Notation "'tyExpr'" := (tyArr tyStack tyVal).
-Notation "'tyFields'" := (tyList tyString).
-
-Notation "'tyVarList'" := (tyList tyString).
-Notation "'tyDExprList'" := (tyList tyDExpr).
-Notation "'tySubstList'" := (tyList (tyProd tyString tyExpr)).
-
-Fixpoint type_cast_typ (a b : typ) : option (a = b) :=
-  match a as a , b as b return option (a = b) with
-    | tyProp , tyProp => Some eq_refl
-    | tySpec , tySpec => Some eq_refl
-    | tyVal, tyVal => Some eq_refl
-    | tyBool, tyBool => Some eq_refl
-    | tyProg, tyProg => Some eq_refl
-    | tyNat, tyNat => Some eq_refl
-    | tyArr x y , tyArr a b =>
-      match type_cast_typ x a , type_cast_typ y b with
-        | Some pf , Some pf' =>
-          Some (match pf in _ = t
-                    , pf' in _ = t'
-                      return tyArr x y = tyArr t t'
-                with
-                  | eq_refl , eq_refl => eq_refl
-                end)
-        | _ , _ => None
-      end
-    | tyProd x y , tyProd a b =>
-      match type_cast_typ x a , type_cast_typ y b with
-        | Some pf , Some pf' =>
-          Some (match pf in _ = t
-                    , pf' in _ = t'
-                      return tyProd x y = tyProd t t'
-                with
-                  | eq_refl , eq_refl => eq_refl
-                end)
-        | _ , _ => None
-      end
-    | tyList x, tyList y =>
-    	match type_cast_typ x y with
-          | Some pf =>
-    		Some (match pf in _ = t return tyList x = tyList t with
-    			    | eq_refl => eq_refl
-    			  end)
-          | None => None
-       end
-    | tyString, tyString => Some eq_refl
-    | tyCmd, tyCmd => Some eq_refl
-    | tyMethod, tyMethod => Some eq_refl
-    | tyDExpr, tyDExpr => Some eq_refl
-    | tyAsn, tyAsn => Some eq_refl
-    | tySubst, tySubst => Some eq_refl
-
-    | _, _ => None
-  end.
-
-Lemma type_cast_typ_sound (a b : typ) :
-	(exists pf, type_cast_typ a b = Some pf) <->
-	a = b.
-Proof.
-  split; intros H.
-  + destruct a, b; destruct H as [x _]; inversion x; subst; reflexivity.
-  + subst. exists eq_refl. induction b; try reflexivity.
-    simpl. rewrite IHb1, IHb2. reflexivity.
-    simpl. rewrite IHb. reflexivity.
-    simpl. rewrite IHb1, IHb2. reflexivity.
-Qed.
-
-Instance RelDec_eq_typ : RelDec (@eq typ) :=
-{ rel_dec := fun a b => match type_cast_typ a b with
-                          | None => false
-                          | Some _ => true
-                        end }.
-
-Lemma type_cast_typ_refl (a : typ) : type_cast_typ a a = Some eq_refl.
-Proof.
-  induction a; simpl; try reflexivity.
-  rewrite IHa1, IHa2; reflexivity.
-  rewrite IHa. reflexivity.
-  rewrite IHa1, IHa2; reflexivity.
-Qed.
-
-Instance RelDec_correct_typ : RelDec_Correct RelDec_eq_typ.
-Proof.
-	split; intros x y.
-	destruct x, y; simpl; split; intro H; inversion H; subst; try reflexivity.
-	+ remember (type_cast_typ x1 y1); destruct o; subst; [|inversion H].
-	  remember (type_cast_typ x2 y2); destruct o; subst; [|inversion H].
-	  reflexivity.
-	+ do 2 rewrite type_cast_typ_refl; reflexivity.
-	+ remember (type_cast_typ x y); destruct o; subst; [|inversion H].
-	  reflexivity.
-	+ rewrite type_cast_typ_refl. reflexivity.
-	+ remember (type_cast_typ x1 y1); destruct o; subst; [|inversion H].
-	  remember (type_cast_typ x2 y2); destruct o; subst; [|inversion H].
-	  reflexivity.
-	+ do 2 rewrite type_cast_typ_refl; reflexivity.
-Qed.
-
-Fixpoint typD (t : typ) : Type :=
-  match t with
-    | tyArr a b => typD a -> typD b
-    | tyList a => @list (typD a)
-    | tyProd a b => (typD a * typD b)%type
-    | tyProp => Prop
-    | tyNat => nat
-    | tyBool => bool
-    | tySpec => spec
-    | tyAsn => asn
-    | tyVal => val
-    | tyString => string
-    | tyProg => Program
-    | tyMethod => Method
-    | tyCmd => cmd
-    | tyDExpr => dexpr
-    | tySubst => @subst var val
-  end.
-
-Inductive tyAcc_typ : typ -> typ -> Prop :=
-| tyAcc_tyArrL : forall a b, tyAcc_typ a (tyArr a b)
-| tyAcc_tyArrR : forall a b, tyAcc_typ a (tyArr b a)
-| tyAcc_tyProdL : forall a b, tyAcc_typ a (tyProd a b)
-| tyAcc_tyProdR : forall a b, tyAcc_typ a (tyProd b a)
-| tyAcc_tyList : forall a, tyAcc_typ a (tyList a).
-
-Global Instance RType_typ : RType typ :=
-{ typD := typD
-; tyAcc := tyAcc_typ
-; type_cast := type_cast_typ
-}.
-
-Global Instance Typ2_Fun : Typ2 _ RFun :=
-{ typ2 := tyArr
-; typ2_cast := fun _ _ => eq_refl
-; typ2_match := fun T t tr =>
-                  match t as t return T (typD t) -> T (typD t) with
-                    | tyArr a b => fun _ => tr a b
-                    | _ => fun fa => fa
-                  end
-}.
-
-Global Instance Typ2Ok_Fun : Typ2Ok Typ2_Fun.
-Proof.
-  split; intros.
-  + reflexivity.
-  + apply (tyAcc_tyArrL).
-  + apply (tyAcc_tyArrR).
-  + unfold Rty in *. inversion H; subst; intuition congruence.
-  + destruct x; try solve [right; reflexivity].
-    left; exists x1, x2, eq_refl. reflexivity.
-  + destruct pf; reflexivity.
-Qed.
-
-Global Instance Typ2_prod : Typ2 _ prod :=
-{ typ2 := tyProd
-; typ2_cast := fun _ _ => eq_refl
-; typ2_match := fun T t tr =>
-                  match t as t return T (typD t) -> T (typD t) with
-                    | tyProd a b => fun _ => tr a b
-                    | _ => fun fa => fa
-                  end
-}.
-
-Global Instance Typ2Ok_prod : Typ2Ok Typ2_prod.
-Proof.
-  split; intros.
-  + reflexivity.
-  + apply (tyAcc_tyProdL).
-  + apply tyAcc_tyProdR.
-  + unfold Rty in *. inversion H; subst; intuition congruence.
-  + destruct x; try solve [right; reflexivity].
-    left; exists x1, x2, eq_refl. reflexivity.
-  + destruct pf; reflexivity.
-Qed.
-
-Global Instance Typ1_list : Typ1 _ list :=
-{ typ1 := tyList
-; typ1_cast := fun _ => eq_refl
-; typ1_match := fun T t tr =>
-                  match t as t return T (typD t) -> T (typD t) with
-                    | tyList a => fun _ => tr a
-                    | _ => fun fa => fa
-                  end
-}.
-
-Global Instance Typ1Ok_list : Typ1Ok Typ1_list.
-Proof.
-  split; intros.
-  + reflexivity.
-  + apply (tyAcc_tyList).
-  + unfold Rty in *. inversion H; subst; intuition congruence.
-  + destruct x; try solve [right; reflexivity].
-    left; exists x, eq_refl. reflexivity.
-  + destruct pf; reflexivity.
-Qed.
-
-Instance Typ0_Prop : Typ0 _ Prop :=
-{ typ0 := tyProp
-; typ0_cast := eq_refl
-; typ0_match := fun T t tr =>
-                  match t as t return T (typD t) -> T (typD t) with
-                    | tyProp => fun _ => tr
-                    | _ => fun fa => fa
-                  end
-}.
-
-Instance Typ0Ok_Prop : Typ0Ok Typ0_Prop.
-Proof.
-    constructor.
-    { reflexivity. }
-    { destruct x; try solve [ right ; reflexivity ].
-      { left. exists eq_refl. reflexivity. } }
-    { destruct pf. reflexivity. }
-Qed.
-
-Instance Typ0_nat : Typ0 _ nat :=
-{ typ0 := tyNat
-; typ0_cast := eq_refl
-; typ0_match := fun T t tr =>
-                  match t as t return T (typD t) -> T (typD t) with
-                    | tyNat => fun _ => tr
-                    | _ => fun fa => fa
-                  end
-}.
-
-Instance Typ0Ok_nat : Typ0Ok Typ0_nat.
-Proof.
-    constructor.
-    { reflexivity. }
-    { destruct x; try solve [ right ; reflexivity ].
-      { left. exists eq_refl. reflexivity. } }
-    { destruct pf. reflexivity. }
-Qed.
-
-Instance Typ0_bool : Typ0 _ bool :=
-{ typ0 := tyBool
-; typ0_cast := eq_refl
-; typ0_match := fun T t tr =>
-                  match t as t return T (typD t) -> T (typD t) with
-                    | tyBool => fun _ => tr
-                    | _ => fun fa => fa
-                  end
-}.
-
-Instance Typ0Ok_bool : Typ0Ok Typ0_bool.
-Proof.
-    constructor.
-    { reflexivity. }
-    { destruct x; try solve [ right ; reflexivity ].
-      { left. exists eq_refl. reflexivity. } }
-    { destruct pf. reflexivity. }
-Qed.
-
-Instance Typ0_string : Typ0 _ string :=
-{ typ0 := tyString
-; typ0_cast := eq_refl
-; typ0_match := fun T t tr =>
-                  match t as t return T (typD t) -> T (typD t) with
-                    | tyString => fun _ => tr
-                    | _ => fun fa => fa
-                  end
-}.
-
-Instance Typ0Ok_string : Typ0Ok Typ0_string.
-Proof.
-    constructor.
-    { reflexivity. }
-    { destruct x; try solve [ right ; reflexivity ].
-      { left. exists eq_refl. reflexivity. } }
-    { destruct pf. reflexivity. }
-Qed.
-
-Instance Typ0_val : Typ0 _ val :=
-{ typ0 := tyVal
-; typ0_cast := eq_refl
-; typ0_match := fun T t tr =>
-                  match t as t return T (typD t) -> T (typD t) with
-                    | tyVal => fun _ => tr
-                    | _ => fun fa => fa
-                  end
-}.
-
-Instance Typ0Ok_val : Typ0Ok Typ0_val.
-Proof.
-    constructor.
-    { reflexivity. }
-    { destruct x; try solve [ right ; reflexivity ].
-      { left. exists eq_refl. reflexivity. } }
-    { destruct pf. reflexivity. }
-Qed.
-
-Instance RTypeOk_typ : @RTypeOk _ RType_typ.
-Proof.
-  split; intros.
-  + reflexivity.
-  + unfold well_founded.
-    intros. induction a; simpl; constructor; intros; inversion H; subst; assumption.
-  + destruct pf; reflexivity.
-  + destruct pf1, pf2; reflexivity.
-  + apply type_cast_typ_refl.
-  + intro H1. inversion H1; subst.
-    rewrite type_cast_typ_refl in H. inversion H.
-  + intros x.
-    induction x; intros y; destruct y; try (right; congruence); try (left; congruence).
-    * destruct (IHx1 y1) as [Hx1 | Hx1]; clear IHx1;
-      destruct (IHx2 y2) as [Hx2 | Hx2]; clear IHx2;
-      try (right; congruence); try (left; congruence).
-    * destruct (IHx y) as [Hx | Hx]; clear IHx; [
-	left; congruence | right; congruence].
-    * destruct (IHx1 y1) as [Hx1 | Hx1]; clear IHx1;
-      destruct (IHx2 y2) as [Hx2 | Hx2]; clear IHx2;
-      try (right; congruence); try (left; congruence).
-Qed.
-
-
-Definition null' : TypesI.typD tyVal := null.
-(*
-Program Instance SubstTypeD_typ : @SubstTypeD typ _ _ _ := {
-	stSubst := eq_refl
-}.
-*)
-Definition should_not_be_necessary : ILogicOps (TypesI.typD tySpec).
-Proof.
-  simpl.
-  apply _.
-Defined.
-
-Definition should_also_not_be_necessary : ILLOperators (TypesI.typD tySpec).
-Proof.
-  simpl.
-  apply _.
-Defined.
-
-  Definition ilops : @logic_ops _ RType_typ :=
-  fun t =>
-    match t
-          return _option (ILogic.ILogicOps (TypesI.typD t))
-    with
-      | tyProp => _Some _
-      | tyAsn => _Some _
-      | tySasn => _Some (@ILFun_Ops stack asn _)
-      | tySpec => _Some should_not_be_necessary
-      | tyPure => _Some (@ILFun_Ops stack Prop _)
-      | _ => _None _
-    end.
-
-  Definition bilops : @bilogic_ops _ RType_typ :=
-  fun t =>
-    match t
-          return option (BILogic.BILOperators (TypesI.typD t))
-    with
-      | tyAsn => Some _
-      | tySasn => Some (@BILFun_Ops stack asn _)
-      | _ => None
-    end.
-
-Definition eops : @embed_ops _ RType_typ :=
-  fun t u =>
-    match t as t , u as u
-          return option
-                   (ILEmbed.EmbedOp (TypesI.typD t) (TypesI.typD u))
-    with
-      | tyPure, tySasn => Some _
-      | tyProp, tyAsn => Some _
-      | _ , _ => None
-    end.
-(*
-Definition lops : @later_ops _ RType_typ :=
-  fun t =>
-    match t return option (ILLOperators (TypesI.typD t)) with
-	  | tySpec => Some should_also_not_be_necessary
-	  | _ => None
-    end.
-*)
-Definition ilp : il_pointwise :=
-  fun t =>
-    match t with
-      | tySasn => true
-      | tyPure => true
-      | _ => false
-    end.
-
-Definition bilp : bil_pointwise :=
-  fun t =>
-    match t with
-      | tySasn => true
-      | _ => false
-    end.
-
-Definition eilp : eil_pointwise :=
-  fun t u =>
-    match t, u with
-      | tyStack, tyProp => true
-      | tyStack, tyAsn => true
-      | _, _ => false
-    end.
-(*
-Lemma eilpOk : eil_pointwiseOk eops eilp.
-Proof.
-  intros t u; simpl.
-  destruct t; try apply I.
-  destruct u; try apply I.
-  remember (type_cast_typ t1 u1).
-  destruct o; try apply I.
-  destruct t1; subst.
-  destruct t1_1.
-  Focus 6.
-  destruct t1_2.
-  Focus 5.
-  destruct t2.
-  Focus 8.
-  destruct u2.
-  Focus 10.
-  match goal with
-    |- match ?a with | Some _ => _ | None => _ end => remember a
-  end.
-  destruct o.
-  intros.
-  pose proof eilf_pointwise_embed_eq (gs := eops) (eilp := eilp).
-  rewrite @eilf_pointwise_embed_eq.
-  simpl. reflexivity.
-  Print il_pointwiseOk.
-  simpl.
-  unfold Denotation.tyArrD, Denotation.tyArrD', Denotation.trmD, Denotation.tyArrR, Denotation.tyArrR', Denotation.trmR, eq_rect_r, eq_rect, eq_sym, id.
-  simpl.
-  unfold ILEmbed.embed.
-  simpl.
-  destruct e.
-  simpl. reflexivity.
-  reflexivity.
-  remember (eops tyProp tySasn).
-  destruct o.
-  rewrite <- Heqo0.
-Print eil_pointwiseOk.
-*)
-(*
-Lemma ilpOk : il_pointwiseOk ilops ilp.
-Proof.
-  intros t; simpl; destruct t; try apply I.
-  destruct t1; simpl; try apply I.
-  destruct t1_1; try apply I.
-  destruct t1_2; try apply I.
-  destruct t2; simpl; try apply I.
-  repeat split.
-  repeat split.
-Qed.
-
-Lemma BilpOk : bil_pointwiseOk bilops bilp.
-Proof.
-  intros t; simpl; destruct t; try apply I.
-  destruct t1; simpl; try apply I.
-  destruct t1_1; try apply I.
-  destruct t1_2; try apply I.
-  destruct t2; simpl; try apply I.
-  repeat split.
-Qed.
-*)
-Fixpoint edt (t : typ) : typD t -> typD t -> option bool :=
-  match t return typD t -> typD t -> option bool with
-    | tyBool => fun e1 e2 => Some (e1 ?[ eq ] e2)
-    | tyVal => fun e1 e2 => Some (e1 ?[ eq ] e2)
-    | tyString => fun e1 e2 => Some (e1 ?[ eq ] e2)
-    | tyNat => fun e1 e2 => Some (e1 ?[ eq ] e2)
-    | tyProg => fun e1 e2 => Some (e1 ?[ eq ] e2)
-    | tyCmd => fun e1 e2 => Some (e1 ?[ eq ] e2)
-    | tyDExpr => fun e1 e2 => Some (e1 ?[ eq ] e2)
-    | tyList tyString => fun e1 e2 => Some (e1 ?[ eq ] e2)
-    | tyProd t1 t2 =>
-      fun e1 e2 =>
-        match edt t1 (fst e1) (fst e2), edt t2 (snd e1) (snd e2) with
-          | Some a, Some b => Some (a && b)
-          | _, _ => None
+Definition java_typ_dec {n} (a : java_typ n) : forall b, {a = b} + {a <> b}.
+  refine(
+    match a as a in java_typ n return forall b : java_typ n, {a = b} + {a <> b} with
+    | tVal =>
+      fun b =>
+        match b as b in java_typ 0 return {tVal = b} + {tVal <> b} with
+        | tVal => left eq_refl
+        | _ => right (fun pf => _)
         end
-    | _ => fun _ _ => None
+    | tSpec =>
+      fun b =>
+        match b as b in java_typ 0 return {tSpec = b} + {tSpec <> b} with
+        | tSpec => left eq_refl
+        | _ => right (fun pf => _)
+        end
+    | tAsn =>
+      fun b =>
+        match b as b in java_typ 0 return {tAsn = b} + {tAsn <> b} with
+        | tAsn => left eq_refl
+        | _ => right (fun pf => _)
+        end
+    | tProg =>
+      fun b =>
+        match b as b in java_typ 0 return {tProg = b} + {tProg <> b} with
+        | tProg => left eq_refl
+        | _ => right (fun pf => _)
+        end
+    | tMethod =>
+      fun b =>
+        match b as b in java_typ 0 return {tMethod = b} + {tMethod <> b} with
+        | tMethod => left eq_refl
+        | _ => right (fun pf => _)
+        end
+    | tCmd =>
+      fun b =>
+        match b as b in java_typ 0 return {tCmd = b} + {tCmd <> b} with
+        | tCmd => left eq_refl
+        | _ => right (fun pf => _)
+        end
+    | tExpr =>
+      fun b =>
+        match b as b in java_typ 0 return {tExpr = b} + {tExpr <> b} with
+        | tExpr => left eq_refl
+        | _ => right (fun pf => _)
+        end
+    | tSubst =>
+      fun b =>
+        match b as b in java_typ 0 return {tSubst = b} + {tSubst <> b} with
+        | tSubst => left eq_refl
+        | _ => right (fun pf => _)
+        end
+    end);  clear -pf; inversion pf.
+Defined.
+
+Definition java_typD {n} (t : java_typ n) : type_for_arity n :=
+  match t with
+  | tVal => val
+  | tSpec => spec
+  | tAsn => asn
+  | tProg => Program
+  | tMethod => Method
+  | tCmd => cmd
+  | tExpr => dexpr
+  | tSubst => @subst var val
   end.
-(*
-Instance SemiEqDecTyp_edt : SemiEqDecTyp typ := {
-    semi_eq_dec_typ := edt
-  }.
 
-Definition edtOk : 
-  forall t a b,
-    match edt t a b with
-      | Some true => a = b
-      | Some false => a <> b
-      | None => True
-    end.
-Proof.
-  induction t; simpl in *; intros; try apply I; try (consider (e1 ?[ eq ] e2); intuition congruence).
-  destruct t; simpl in *; try apply I.
-  consider (a ?[ eq ] b); intuition congruence.
-  destruct a, b; simpl.
-  forward. inv_all; subst. 
-  specialize (IHt1 t t3); specialize (IHt2 t0 t4).
-  destruct b0, b1; rewrite H in IHt1; rewrite H0 in IHt2; simpl; intuition congruence.
-  consider (a ?[ eq ] b); intuition congruence.
-  consider (a ?[ eq ] b); intuition congruence.
-  consider (a ?[ eq ] b); intuition congruence.
-  consider (a ?[ eq ] b); intuition congruence.
-  consider (a ?[ eq ] b); intuition congruence.
-  consider (a ?[ eq ] b); intuition congruence.
-  consider (a ?[ eq ] b); intuition congruence.
-Qed.
 
-Instance SemiEqDecTypOk_edt : SemiEqDecTypOk SemiEqDecTyp_edt := {
-    semi_eq_dec_typOk := edtOk
-  }.
+Section FuncView_java_type.
+  Context {typ : Type}.
+  Context {FV : FuncView typ (java_typ 0)}.
 
-*)
+  Definition tyVal := f_insert tVal.
+  Definition tySpec := f_insert tSpec.
+  Definition tyAsn := f_insert tAsn.
+  Definition tyProg := f_insert tProg.
+  Definition tyMethod := f_insert tMethod.
+  Definition tyCmd := f_insert tCmd.
+  Definition tyExpr := f_insert tExpr.
+  Definition tySubst := f_insert tSubst.
+
+End FuncView_java_type.
