Java/src/Java/Func/Type.v
@@ -1,0 +1,377 @@
+Require Import ExtLib.Core.RelDec.
+Require Import ExtLib.Data.Fun.
+Require Import ExtLib.Data.POption.
+Require Import ExtLib.Tactics.
+
+Require Import MirrorCore.TypesI.
+Require Import MirrorCore.MTypes.ModularTypes.
+Require Import MirrorCore.MTypes.ListType.
+Require Import MirrorCore.MTypes.ProdType.
+Require Import MirrorCore.MTypes.BaseType.
+Require Import MirrorCore.syms.SymOneOf.
+Require Import MirrorCore.Views.FuncView.
+Require Import MirrorCore.Views.ViewSumN.
+Require Import Java.Func.BaseType.
+Require Import Java.Func.ProdType.
+Require Import MirrorCore.MTypes.ListType.
+
+Require Import Charge.Views.ILogicView.
+Require Import Charge.Views.BILogicView.
+Require Import Charge.Views.EmbedView.
+Require Import ChargeCore.Open.Subst.
+Require Import ChargeCore.Logics.ILInsts.
+Require Import ChargeCore.Logics.BILInsts.
+Require Import ChargeCore.Logics.ILogic.
+Require Import ChargeCore.Logics.Later.
+
+Require Import Java.Logic.AssertionLogic.
+Require Import Java.Logic.SpecLogic.
+Require Import Java.Language.Lang.
+Require Import Java.Language.Program.
+Require Import Java.Func.JavaType.
+
+Require Import Coq.Strings.String.
+Require Import Coq.Bool.Bool.
+
+Set Implicit Arguments.
+Set Strict Implicit.
+
+Import OneOfType.
+
+Definition typ_map x := 
+  list_to_pmap 
+    (prod_typ x :: 
+     list_typ x :: 
+     base_typ x :: 
+     java_typ x :: 
+     nil).
+
+Definition typ' x := OneOfType.OneOf (typ_map x).
+Definition typ := mtyp typ'.
+
+Ltac pmap_lookup'_simpl :=
+  repeat (
+    match goal with 
+    | H : match pmap_lookup' Empty ?p with | _Some _ => _ | _None => Empty_set end |- _ => 
+      exfalso; clear -H; rewrite pmap_lookup'_Empty in H; destruct H
+    | H : match pmap_lookup' _ ?p with | _Some _ => _ | _None => Empty_set end |- _ => 
+      destruct p; simpl in H
+    end).
+
+Ltac eq_dec_right :=
+  let H := fresh "H" in
+    right; intro H; inv_all; congruence.
+
+Definition typ'_dec {n} (a : typ' n) : forall b, {a = b} + {a <> b}.
+Proof.
+  intros.
+  destruct a as [a1 v1].
+  destruct b as [a2 v2].
+  unfold typ_map, list_to_pmap in *. simpl in *.
+  pmap_lookup'_simpl; try eq_dec_right.  
+  pose proof (base_typ_dec v1 v2).
+  destruct H; [left; subst; reflexivity|].
+  right; intros H; apply n0; inv_all; subst.
+  assert (x = eq_refl) by (apply UIP_refl); subst. reflexivity.
+  pose proof (java_typ_dec v1 v2).
+  destruct H; [left; subst; reflexivity|].
+  right; intros H; apply n0; inv_all; subst.
+  assert (x = eq_refl) by (apply UIP_refl); subst. reflexivity.
+  pose proof (list_typ_dec v1 v2).
+  destruct H; [left; subst; reflexivity|].
+  right; intros H; apply n0; inv_all; subst.
+  assert (x = eq_refl) by (apply UIP_refl); subst. reflexivity.
+  pose proof (prod_typ_dec v1 v2).
+  destruct H; [left; subst; reflexivity|].
+  right; intros H; apply n0; inv_all; subst.
+  assert (x = eq_refl) by (apply UIP_refl); subst. reflexivity.
+Defined.
+
+Definition typ'D {n} (t : typ' n) : type_for_arity n.
+unfold typ', typ_map, list_to_pmap in t; simpl in t.
+destruct t as [p v].
+pmap_lookup'_simpl.
+apply base_typD; assumption.
+apply java_typD; assumption.
+apply list_typD; assumption.
+apply prod_typD; assumption.
+Defined.
+
+
+Global Instance TypeView_prod_typ' : FuncView (typ' 2) (prod_typ 2) :=
+  FuncViewPMap 1 (typ_map 2) eq_refl.
+  
+Global Instance TypeView_list_typ' : FuncView (typ' 1) (list_typ 1) :=
+  FuncViewPMap 2 (typ_map 1) eq_refl.
+  
+Global Instance TypeView_base_typ' : FuncView (typ' 0) (base_typ 0) :=
+  FuncViewPMap 3 (typ_map 0) eq_refl.
+  
+Global Instance TypeView_java_typ' : FuncView (typ' 0) (java_typ 0) :=
+  FuncViewPMap 4 (typ_map 0) eq_refl.
+  
+Instance TypeView_prod_typ : FuncView typ (prod_typ 2 * typ * typ).
+eapply FuncView_trans. 
+apply FuncView_sym2.
+eapply (@FuncView_prod _ _ _ _ (@FuncView_prod _ _ _ _ _ FuncView_id) FuncView_id). 
+Defined.
+
+Instance TypeView_list_typ : FuncView typ (list_typ 1 * typ).
+eapply FuncView_trans. 
+apply FuncView_sym1.
+eapply (@FuncView_prod _ _ _ _ _ FuncView_id). 
+Defined.
+
+Instance TypeView_base_typ : FuncView typ (base_typ 0).
+eapply FuncView_trans. 
+eapply FuncView_sym0.
+apply TypeView_base_typ'.
+Defined.
+
+Instance TypeView_java_typ : FuncView typ (java_typ 0).
+eapply FuncView_trans. 
+eapply FuncView_sym0.
+apply TypeView_java_typ'.
+Defined.
+
+Notation "'tyStack'" := (tyArr tyString tyVal).
+
+Notation "'tyPure'" := (tyArr tyStack tyProp).
+Notation "'tySasn'" := (tyArr tyStack tyAsn).
+Notation "'tyExpr'" := (tyArr tyStack tyVal).
+Notation "'tyFields'" := (tyList tyString).
+
+Notation "'tyVarList'" := (tyList tyString).
+Notation "'tyDExprList'" := (tyList tyExpr).
+Notation "'tySubstList'" := (tyList (tyProd tyString tyExpr)).
+
+Instance TSym_typ' : TSym typ' := { 
+  symbolD := @typ'D; 
+  symbol_dec := @typ'_dec 
+}.
+
+
+(* Instantiate the RType interface *)
+Instance RType_typ : RType typ := RType_mtyp typ' _.
+Instance RTypeOk_typ : RTypeOk := @RTypeOk_mtyp typ' _.
+
+(* Build instances for describing functions and Prop *)
+Instance Typ2_tyArr : Typ2 RType_typ Fun := Typ2_Fun.
+Instance Typ2Ok_tyArr : Typ2Ok Typ2_tyArr := Typ2Ok_Fun.
+
+Instance Typ0_tyProp : Typ0 RType_typ Prop := Typ0_sym tyProp.
+Instance Typ0Ok_tyProp : Typ0Ok Typ0_tyProp := Typ0Ok_sym tyProp.
+
+Instance Typ0_tyNat : Typ0 RType_typ nat := Typ0_sym tyNat.
+Instance Typ0Ok_tyNat : Typ0Ok Typ0_tyNat := Typ0Ok_sym tyNat.
+
+Instance Typ0_tyString : Typ0 RType_typ string := Typ0_sym tyString.
+Instance Typ0Ok_tyString : Typ0Ok Typ0_tyString := Typ0Ok_sym tyString.
+
+Instance Typ0_tyBool : Typ0 RType_typ bool := Typ0_sym tyBool.
+Instance Typ0Ok_tyBool : Typ0Ok Typ0_tyBool := Typ0Ok_sym tyBool.
+
+Instance Typ1_tyList : Typ1 RType_typ list := Typ1_sym (f_insert tList).
+Instance Typ1Ok_tyList : Typ1Ok Typ1_tyList := Typ1Ok_sym (f_insert tList).
+
+Instance Typ2_tyProd : Typ2 RType_typ prod := Typ2_sym (f_insert tProd).
+Instance Typ2Ok_tyProd : Typ2Ok Typ2_tyProd := Typ2Ok_sym (f_insert tProd).
+
+
+
+(* 
+
+Definition null' : TypesI.typD tyVal := null.
+(*
+Program Instance SubstTypeD_typ : @SubstTypeD typ _ _ _ := {
+	stSubst := eq_refl
+}.
+*)
+Definition should_not_be_necessary : ILogicOps (TypesI.typD tySpec).
+Proof.
+  simpl.
+  apply _.
+Defined.
+
+Definition should_also_not_be_necessary : ILLOperators (TypesI.typD tySpec).
+Proof.
+  simpl.
+  apply _.
+Defined.
+
+  Definition ilops : @logic_ops _ RType_typ :=
+  fun t =>
+    match t
+          return _option (ILogic.ILogicOps (TypesI.typD t))
+    with
+      | tyProp => _Some _
+      | tyAsn => _Some _
+      | tySasn => _Some (@ILFun_Ops stack asn _)
+      | tySpec => _Some should_not_be_necessary
+      | tyPure => _Some (@ILFun_Ops stack Prop _)
+      | _ => _None _
+    end.
+
+  Definition bilops : @bilogic_ops _ RType_typ :=
+  fun t =>
+    match t
+          return option (BILogic.BILOperators (TypesI.typD t))
+    with
+      | tyAsn => Some _
+      | tySasn => Some (@BILFun_Ops stack asn _)
+      | _ => None
+    end.
+
+Definition eops : @embed_ops _ RType_typ :=
+  fun t u =>
+    match t as t , u as u
+          return option
+                   (ILEmbed.EmbedOp (TypesI.typD t) (TypesI.typD u))
+    with
+      | tyPure, tySasn => Some _
+      | tyProp, tyAsn => Some _
+      | _ , _ => None
+    end.
+(*
+Definition lops : @later_ops _ RType_typ :=
+  fun t =>
+    match t return option (ILLOperators (TypesI.typD t)) with
+	  | tySpec => Some should_also_not_be_necessary
+	  | _ => None
+    end.
+*)
+Definition ilp : il_pointwise :=
+  fun t =>
+    match t with
+      | tySasn => true
+      | tyPure => true
+      | _ => false
+    end.
+
+Definition bilp : bil_pointwise :=
+  fun t =>
+    match t with
+      | tySasn => true
+      | _ => false
+    end.
+
+Definition eilp : eil_pointwise :=
+  fun t u =>
+    match t, u with
+      | tyStack, tyProp => true
+      | tyStack, tyAsn => true
+      | _, _ => false
+    end.
+(*
+Lemma eilpOk : eil_pointwiseOk eops eilp.
+Proof.
+  intros t u; simpl.
+  destruct t; try apply I.
+  destruct u; try apply I.
+  remember (type_cast_typ t1 u1).
+  destruct o; try apply I.
+  destruct t1; subst.
+  destruct t1_1.
+  Focus 6.
+  destruct t1_2.
+  Focus 5.
+  destruct t2.
+  Focus 8.
+  destruct u2.
+  Focus 10.
+  match goal with
+    |- match ?a with | Some _ => _ | None => _ end => remember a
+  end.
+  destruct o.
+  intros.
+  pose proof eilf_pointwise_embed_eq (gs := eops) (eilp := eilp).
+  rewrite @eilf_pointwise_embed_eq.
+  simpl. reflexivity.
+  Print il_pointwiseOk.
+  simpl.
+  unfold Denotation.tyArrD, Denotation.tyArrD', Denotation.trmD, Denotation.tyArrR, Denotation.tyArrR', Denotation.trmR, eq_rect_r, eq_rect, eq_sym, id.
+  simpl.
+  unfold ILEmbed.embed.
+  simpl.
+  destruct e.
+  simpl. reflexivity.
+  reflexivity.
+  remember (eops tyProp tySasn).
+  destruct o.
+  rewrite <- Heqo0.
+Print eil_pointwiseOk.
+*)
+(*
+Lemma ilpOk : il_pointwiseOk ilops ilp.
+Proof.
+  intros t; simpl; destruct t; try apply I.
+  destruct t1; simpl; try apply I.
+  destruct t1_1; try apply I.
+  destruct t1_2; try apply I.
+  destruct t2; simpl; try apply I.
+  repeat split.
+  repeat split.
+Qed.
+
+Lemma BilpOk : bil_pointwiseOk bilops bilp.
+Proof.
+  intros t; simpl; destruct t; try apply I.
+  destruct t1; simpl; try apply I.
+  destruct t1_1; try apply I.
+  destruct t1_2; try apply I.
+  destruct t2; simpl; try apply I.
+  repeat split.
+Qed.
+*)
+Fixpoint edt (t : typ) : typD t -> typD t -> option bool :=
+  match t return typD t -> typD t -> option bool with
+    | tyBool => fun e1 e2 => Some (e1 ?[ eq ] e2)
+    | tyVal => fun e1 e2 => Some (e1 ?[ eq ] e2)
+    | tyString => fun e1 e2 => Some (e1 ?[ eq ] e2)
+    | tyNat => fun e1 e2 => Some (e1 ?[ eq ] e2)
+    | tyProg => fun e1 e2 => Some (e1 ?[ eq ] e2)
+    | tyCmd => fun e1 e2 => Some (e1 ?[ eq ] e2)
+    | tyDExpr => fun e1 e2 => Some (e1 ?[ eq ] e2)
+    | tyList tyString => fun e1 e2 => Some (e1 ?[ eq ] e2)
+    | tyProd t1 t2 =>
+      fun e1 e2 =>
+        match edt t1 (fst e1) (fst e2), edt t2 (snd e1) (snd e2) with
+          | Some a, Some b => Some (a && b)
+          | _, _ => None
+        end
+    | _ => fun _ _ => None
+  end.
+(*
+Instance SemiEqDecTyp_edt : SemiEqDecTyp typ := {
+    semi_eq_dec_typ := edt
+  }.
+
+Definition edtOk : 
+  forall t a b,
+    match edt t a b with
+      | Some true => a = b
+      | Some false => a <> b
+      | None => True
+    end.
+Proof.
+  induction t; simpl in *; intros; try apply I; try (consider (e1 ?[ eq ] e2); intuition congruence).
+  destruct t; simpl in *; try apply I.
+  consider (a ?[ eq ] b); intuition congruence.
+  destruct a, b; simpl.
+  forward. inv_all; subst. 
+  specialize (IHt1 t t3); specialize (IHt2 t0 t4).
+  destruct b0, b1; rewrite H in IHt1; rewrite H0 in IHt2; simpl; intuition congruence.
+  consider (a ?[ eq ] b); intuition congruence.
+  consider (a ?[ eq ] b); intuition congruence.
+  consider (a ?[ eq ] b); intuition congruence.
+  consider (a ?[ eq ] b); intuition congruence.
+  consider (a ?[ eq ] b); intuition congruence.
+  consider (a ?[ eq ] b); intuition congruence.
+  consider (a ?[ eq ] b); intuition congruence.
+Qed.
+
+Instance SemiEqDecTypOk_edt : SemiEqDecTypOk SemiEqDecTyp_edt := {
+    semi_eq_dec_typOk := edtOk
+  }.
+
+*) *)
